Prepare trees_equal for one-sided read:
* add new assymetric case allowing read on one side
* tweak everything that is broken by it by embracing the assymetricity
* push changes through

What is missing:
Proving that if memory_access AccessRead = None, then it's also None on the other side.
iow reads are still symmetric.
This is needed for handling poison.

Alternatively, we might remove posion, but we should still prove this result.

theories/tree_borrows/logical_state.v
@@ -166,7 +166,7 @@ Section state_bijection.
     *)
     Definition state_rel σ_t σ_s : iProp Σ :=
         ⌜dom σ_s.(shp) = dom σ_t.(shp)⌝ ∗
-        ⌜trees_equal σ_s.(scs) σ_s.(strs) σ_t.(strs)⌝ ∗
+        ⌜trees_equal σ_s.(scs) Forwards σ_s.(strs) σ_t.(strs)⌝ ∗
         ⌜σ_s.(snp) = σ_t.(snp)⌝ ∗
         ⌜σ_s.(snc) = σ_t.(snc)⌝ ∗
         ⌜σ_s.(scs) = σ_t.(scs)⌝ ∗
@@ -185,14 +185,14 @@ Section bijection_lemmas.
   Local Notation state_rel := (state_rel sc_rel).
 
   Lemma state_rel_get_pure Mtag Mt Mcall σ_t σ_s :
-    state_rel Mtag Mt Mcall σ_t σ_s -∗ ⌜trees_equal σ_s.(scs) σ_s.(strs) σ_t.(strs) ∧
+    state_rel Mtag Mt Mcall σ_t σ_s -∗ ⌜trees_equal σ_s.(scs) Forwards σ_s.(strs) σ_t.(strs) ∧
       σ_s.(snp) = σ_t.(snp) ∧ σ_s.(snc) = σ_t.(snc) ∧ σ_s.(scs) = σ_t.(scs)⌝.
   Proof. iIntros "(% & % & % & % & % & ?)". eauto. Qed.
   Lemma state_rel_trees_eq Mtag Mt Mcall σ_t σ_s :
-    state_rel Mtag Mt Mcall σ_t σ_s -∗ ⌜trees_equal σ_s.(scs) σ_s.(strs) σ_t.(strs)⌝.
+    state_rel Mtag Mt Mcall σ_t σ_s -∗ ⌜trees_equal σ_s.(scs) Forwards σ_s.(strs) σ_t.(strs)⌝.
   Proof. iIntros "(% & % & % & % & % & ?)". eauto. Qed.
   Lemma state_rel_trees_eq_2 Mtag Mt Mcall σ_t σ_s :
-    state_rel Mtag Mt Mcall σ_t σ_s -∗ ⌜trees_equal σ_t.(scs) σ_s.(strs) σ_t.(strs)⌝.
+    state_rel Mtag Mt Mcall σ_t σ_s -∗ ⌜trees_equal σ_t.(scs) Forwards σ_s.(strs) σ_t.(strs)⌝.
   Proof. iIntros "(% & % & % & % & <- & ?)". eauto. Qed.
   Lemma state_rel_snp_eq Mtag Mt Mcall σ_t σ_s :
     state_rel Mtag Mt Mcall σ_t σ_s -∗ ⌜σ_s.(snp) = σ_t.(snp)⌝.
@@ -1105,7 +1105,7 @@ Section state_interp.
      bor_interp_inner σ_t σ_s M_call M_tag M_t M_s.
 
   Lemma bor_interp_get_pure σ_t σ_s :
-    bor_interp σ_t σ_s -∗ ⌜trees_equal σ_s.(scs) σ_s.(strs) σ_t.(strs) ∧ σ_s.(snp) = σ_t.(snp) ∧
+    bor_interp σ_t σ_s -∗ ⌜trees_equal σ_s.(scs) Forwards σ_s.(strs) σ_t.(strs) ∧ σ_s.(snp) = σ_t.(snp) ∧
     σ_s.(snc) = σ_t.(snc) ∧ σ_s.(scs) = σ_t.(scs) ∧ state_wf σ_s ∧ state_wf σ_t ∧
     dom σ_s.(shp) = dom σ_t.(shp)⌝.
   Proof.
