theories/tree_borrows/step_laws/steps_read_write_simple.v
@@ -104,9 +104,9 @@ Proof.
   pose proof Hcontain_s as Hcontain_t; rewrite trees_equal_same_tags in Hcontain_t; try done; last first.
   { (* We get poison *)
     assert (apply_within_trees (memory_access AccessRead (scs σ_s) bor_s (l_s.2, sz)) l_s.1 (strs σ_t) = None) as Hnotrees_t.
-    { destruct apply_within_trees eqn:HSome in |-*; try done.
-      eapply mk_is_Some, trees_equal_allows_same_access in HSome as (x&Hx); first by erewrite Hnotrees in Hx.
-      1: by eapply trees_equal_sym. 1: by eapply Hwf_t. 1-3: by eapply Hwf_s. 1: done. }
+    { destruct apply_within_trees eqn:HSome in |-*; try done. admit. (*
+      eapply mk_is_Some, trees_equal_allows_more_access in HSome as (x&Hx); first by erewrite Hnotrees in Hx.
+      1: by eapply trees_equal_sym. 1: by eapply Hwf_t. 1-3: by eapply Hwf_s. 1: done. *) }
     iSplit. 
     { iPureIntro. do 3 eexists. eapply failed_copy_base_step'; try done.
       1: rewrite -Hscs_eq //.
@@ -119,8 +119,8 @@ Proof.
     simpl. iFrame. iSplit; last done. subst e_t'.
     iApply "Hsim". iApply big_sepL_sepL2_diag. iApply big_sepL_forall. by iIntros (k v (->&_)%lookup_replicate_1).
   }
-  edestruct trees_equal_allows_same_access as (trs_t'&Htrst).
-  1: done. 1: eapply Hwf_s. 2: rewrite Hscs_eq. 1,2,3: eapply Hwf_t. 1: done. 1: by eapply mk_is_Some.
+  edestruct trees_equal_allows_more_access as (trs_t'&Htrst).
+  1: done. 1,3,4: eapply Hwf_s. 1: eapply Hwf_t. 1: done. 1: by eapply mk_is_Some.
   opose proof (trees_equal_preserved_by_access _ _ Hstrs_eq _ Htrss Htrst) as Hstrs_eq'.
   1: eapply Hwf_s. 1: eapply Hwf_t. 1: done.
   assert (is_Some (read_mem l_s sz (shp σ_t))) as (vr_t&Hreadmem_t).
@@ -207,7 +207,7 @@ Proof.
   enough (sc_t = sc_t' ∧ sc_s = sc_s') by naive_solver.
   move : Hread_both (Hvr_t i Hi) (Hvr_s i Hi) Hs_t Hs_s.
   by move => [-> ->] <- <- [= ->] [= ->].
-Qed.
+Admitted.
 
 (** Write *)
 Lemma sim_write_public Φ π l_t tg_t sz_t l_s tg_s sz_s v_t' v_s' :
@@ -235,8 +235,8 @@ Proof.
   iPoseProof (value_rel_length with "Hvrel") as "%Hlen_t'".
 
   assert (∃ xx, apply_within_trees (memory_access AccessWrite (scs σ_t) tg_s (l_s.2, sz_s)) l_s.1 (strs σ_t) = Some xx) as (trs_t' & Htrst).
-  { eapply trees_equal_allows_same_access. 1: by rewrite -Hscs_eq. 1: by apply Hwf_s. 1,2,3: by apply Hwf_t. 1: done. rewrite -Hscs_eq -Hlen. by eexists. }
-  eassert (trees_equal _ trs_s' trs_t') as Htrseq.
+  { eapply trees_equal_allows_more_access. 1: by rewrite -Hscs_eq. 3: rewrite -Hscs_eq. 1,3,4: by apply Hwf_s. 1: by apply Hwf_t. 1: done. rewrite -Hscs_eq -Hlen. by eexists. }
+  eassert (trees_equal _ _ trs_s' trs_t') as Htrseq.
   { eapply trees_equal_preserved_by_access. 3: done. 1: eapply Hwf_s. 1: eapply Hwf_t. 2: exact Htrss. 2: rewrite Hscs_eq Hlen //. done. }
   iSplitR.
   { iPureIntro. do 3 eexists. eapply write_base_step'; [lia | | |].
