theories/tree_borrows/step_laws/steps_unique.v
@@ -103,8 +103,8 @@ Proof.
   destruct Htreeorz as [(Hcontain&trs_s'&Htree_s)|?]. 2: done.
 
   eapply mk_is_Some in Htree_s as Htree_t.
-  eapply trees_equal_allows_same_access in Htree_t as (trs_t' & Htree_t);
-    [|done|eapply Hwf_s|eapply Hwf_t|rewrite Hscs_eq; by eapply Hwf_t|by eapply Hwf_t|done].
+  eapply trees_equal_allows_more_access in Htree_t as (trs_t' & Htree_t);
+    [|done|eapply Hwf_s|eapply Hwf_t|by eapply Hwf_s|by eapply Hwf_s|done].
 
   edestruct (trees_equal_same_tags) as [HL _]; first done.
   eapply HL in Hcontain as Hcontain_t; clear HL.
